Began rewrite...

LogicalRefinement/Untyped.lean
@@ -3,482 +3,167 @@
 import Init.Data.Nat
 import LogicalRefinement.Wk
 
-inductive Untyped: Nat -> Type 0 where
-
-  -- Variables
-  | var (m: Fin n): Untyped n
+inductive UntypedKind: Type where
 
   -- Types
-  | nat: Untyped n
-  | pi (A: Untyped n) (B: Untyped (n + 1)): Untyped n
-  | sigma (A: Untyped n) (B: Untyped (n + 1)): Untyped n
-  | coprod (A: Untyped n) (B: Untyped n): Untyped n
-  | set (A: Untyped n) (φ: Untyped (n + 1)): Untyped n
-  | assume (φ: Untyped n) (A: Untyped n): Untyped n
-  | intersect (A: Untyped n) (B: Untyped (n + 1)): Untyped n
-  | union (A: Untyped n) (B: Untyped (n + 1)): Untyped n
+  | nats
+  | pi
+  | sigma
+  | coprod
+  | set
+  | assume
+  | intersect
+  | union
 
   -- Propositions
-  | top: Untyped n
-  | bot: Untyped n
-  | and (φ: Untyped n) (ψ: Untyped n): Untyped n
-  | or (φ: Untyped n) (ψ: Untyped n): Untyped n
-  | implies (φ: Untyped n) (ψ: Untyped n): Untyped n
-  | forall_ (A: Untyped n) (φ: Untyped (n + 1)): Untyped n
-  | exists_ (A: Untyped n) (φ: Untyped (n + 1)): Untyped n
-  | eq (A: Untyped n) (e: Untyped n) (e': Untyped n): Untyped n
+  | top
+  | bot
+  | and
+  | or
+  | implies
+  | forall_
+  | exists_
+  | eq
 
   -- Terms
-  | lam (A: Untyped n) (e: Untyped (n + 1)): Untyped n
-  | app (l: Untyped n) (r: Untyped n): Untyped n
-  | pair (l: Untyped n) (r: Untyped n): Untyped n
-  | proj (b: Bool) (e: Untyped n): Untyped n
-  | inj (b: Bool) (e: Untyped n): Untyped n
-  | case (e: Untyped n) (l: Untyped n) (r: Untyped n): Untyped n
-  | mkset (e: Untyped n) (p: Untyped n): Untyped n
-  | letset (e: Untyped (n + 2)): Untyped n
-  | lam_pr (φ: Untyped n) (e: Untyped (n + 1)): Untyped n
-  | app_pr (e: Untyped n) (p: Untyped n): Untyped n
-  | lam_irrel (A: Untyped n) (e: Untyped (n + 1)): Untyped n
-  | app_irrel (l: Untyped n) (r: Untyped n): Untyped n
-  | repr (l: Untyped n) (r: Untyped n): Untyped n
-  | let_repr (e: Untyped (n + 2)): Untyped n
+  | nat (n: Nat)
+  | lam
+  | app
+  | pair
+  | proj (b: Bool)
+  | inj (b: Bool)
+  | case
+  | mkset
+  | letset
+  | lam_pr
+  | app_pr
+  | lam_irrel
+  | app_irrel
+  | repr
+  | let_repr
 
   -- Proofs
-  | nil: Untyped n
-  | abort (p: Untyped n): Untyped n
-  | conj (l: Untyped n) (r: Untyped n): Untyped n
-  | comp (b: Bool) (p: Untyped n): Untyped n
-  | disj (b: Bool) (p: Untyped n): Untyped n
-  | case_pr (p: Untyped n) (l: Untyped n) (r: Untyped n): Untyped n
-  | imp (φ: Untyped n) (p: Untyped (n + 1)): Untyped n
-  | mp (l: Untyped n) (r: Untyped n): Untyped n
-  | general (A: Untyped n) (p: Untyped (n + 1)): Untyped n
-  | inst (p: Untyped n) (e: Untyped n): Untyped n
-  | witness (e: Untyped n) (p: Untyped n): Untyped n
-  | let_wit (p: Untyped (n + 2)): Untyped n
-  | refl (e: Untyped n): Untyped n
-  --TODO: equality axioms...
+  | nil
+  | abort
+  | conj
+  | comp (b: Bool)
+  | disj (b: Bool)
+  | case_pr
+  | imp
+  | mp
+  | general
+  | inst
+  | witness
+  | let_wit
+  | refl
 
-@[simp] def Fin.succ: Fin n -> Fin (Nat.succ n)
-  | Fin.mk m p => Fin.mk (Nat.succ m) (Nat.lt_succ_of_le p)
-
-@[simp] def Fin.zero: Fin (Nat.succ n) := Fin.mk 0 (Nat.zero_lt_succ _)
-
-def wk (ρ: Wk n m): Untyped m -> Untyped n
+inductive RawUntyped: Type where
 
   -- Variables
-  | Untyped.var m => Untyped.var (Wk.var ρ m)
+  | var (n: Nat)
+
+  -- Base terms
 
   -- Types
-  | Untyped.nat => Untyped.nat
-  | Untyped.pi A B => Untyped.pi (wk ρ A) (wk (Wk.lift ρ) B)
-  | Untyped.sigma A B => Untyped.sigma (wk ρ A) (wk (Wk.lift ρ) B)
-  | Untyped.coprod A B => Untyped.coprod (wk ρ A) (wk ρ B)
-  | Untyped.set A φ => Untyped.set (wk ρ A) (wk (Wk.lift ρ) φ)
-  | Untyped.assume φ A => Untyped.assume (wk ρ φ) (wk ρ A)
-  | Untyped.intersect A B => Untyped.intersect (wk ρ A) (wk (Wk.lift ρ) B)
-  | Untyped.union A B => Untyped.union (wk ρ A) (wk (Wk.lift ρ) B)
+  | nats
+  | pi (A: RawUntyped) (B: RawUntyped)
+  | sigma (A: RawUntyped) (B: RawUntyped)
+  | coprod (A: RawUntyped) (B: RawUntyped)
+  | set (A: RawUntyped) (φ: RawUntyped)
+  | assume (φ: RawUntyped) (A: RawUntyped)
+  | intersect (A: RawUntyped) (B: RawUntyped)
+  | union (A: RawUntyped) (B: RawUntyped)
 
   -- Propositions
-  | Untyped.top => Untyped.top
-  | Untyped.bot => Untyped.bot
-  | Untyped.and φ ψ => Untyped.and (wk ρ φ) (wk ρ ψ)
-  | Untyped.or φ ψ => Untyped.or (wk ρ φ) (wk ρ ψ)
-  | Untyped.implies φ ψ => Untyped.implies (wk ρ φ) (wk ρ ψ)
-  | Untyped.forall_ A φ => Untyped.forall_ (wk ρ A) (wk (Wk.lift ρ) φ)
-  | Untyped.exists_ A φ => Untyped.exists_ (wk ρ A) (wk (Wk.lift ρ) φ)
-  | Untyped.eq A l r => Untyped.eq (wk ρ A) (wk ρ l) (wk ρ r)
-  
+  | top
+  | bot
+  | and (φ: RawUntyped) (ψ: RawUntyped)
+  | or (φ: RawUntyped) (ψ: RawUntyped)
+  | implies (φ: RawUntyped) (ψ: RawUntyped)
+  | forall_ (A: RawUntyped) (φ: RawUntyped)
+  | exists_ (A: RawUntyped) (φ: RawUntyped)
+  | eq (A: RawUntyped) (e: RawUntyped) (e': RawUntyped)
+
   -- Terms
-  | Untyped.lam A e => Untyped.lam (wk ρ A) (wk (Wk.lift ρ) e)
-  | Untyped.app l r => Untyped.app (wk ρ l) (wk ρ r)
-  | Untyped.pair l r => Untyped.pair (wk ρ l) (wk ρ r)
-  | Untyped.proj b e => Untyped.proj b (wk ρ e)
-  | Untyped.inj b e => Untyped.inj b (wk ρ e)
-  | Untyped.case e l r => Untyped.case (wk ρ e) (wk ρ l) (wk ρ r)
-  | Untyped.mkset e p => Untyped.mkset (wk ρ e) (wk ρ p)
-  | Untyped.letset e => Untyped.letset (wk (Wk.liftn 2 ρ) e)
-  | Untyped.lam_pr φ e => Untyped.lam_pr (wk ρ φ) (wk (Wk.lift ρ) e)
-  | Untyped.app_pr φ e => Untyped.app_pr (wk ρ φ) (wk ρ e)
-  | Untyped.lam_irrel l r => Untyped.lam_irrel (wk ρ l) (wk (Wk.lift ρ) r)
-  | Untyped.app_irrel l r => Untyped.app_irrel (wk ρ l) (wk ρ r)
-  | Untyped.repr l r => Untyped.repr (wk ρ l) (wk ρ r)
-  | Untyped.let_repr e => Untyped.let_repr (wk (Wk.liftn 2 ρ) e)
+  | nat (n: Nat)
+  | lam (A: RawUntyped) (e: RawUntyped)
+  | app (l: RawUntyped) (r: RawUntyped)
+  | pair (l: RawUntyped) (r: RawUntyped)
+  | proj (b: Bool) (e: RawUntyped)
+  | inj (b: Bool) (e: RawUntyped)
+  | case (e: RawUntyped) (l: RawUntyped) (r: RawUntyped)
+  | mkset (e: RawUntyped) (p: RawUntyped)
+  | letset (e: RawUntyped)
+  | lam_pr (φ: RawUntyped) (e: RawUntyped)
+  | app_pr (e: RawUntyped) (p: RawUntyped)
+  | lam_irrel (A: RawUntyped) (e: RawUntyped)
+  | app_irrel (l: RawUntyped) (r: RawUntyped)
+  | repr (l: RawUntyped) (r: RawUntyped)
+  | let_repr (e: RawUntyped)
 
   -- Proofs
-  | Untyped.nil => Untyped.nil
-  | Untyped.abort p => Untyped.abort (wk ρ p)
-  | Untyped.conj l r => Untyped.conj (wk ρ l) (wk ρ r)
-  | Untyped.comp b p => Untyped.comp b (wk ρ p)
-  | Untyped.disj b p => Untyped.disj b (wk ρ p)
-  | Untyped.case_pr p l r => Untyped.case_pr (wk ρ p) (wk ρ l) (wk ρ r)
-  | Untyped.imp φ p => Untyped.imp (wk ρ φ) (wk (Wk.lift ρ) p)
-  | Untyped.mp l r => Untyped.mp (wk ρ l) (wk ρ r)
-  | Untyped.general A p => Untyped.general (wk ρ A) (wk (Wk.lift ρ) p)
-  | Untyped.inst p e => Untyped.inst (wk ρ p) (wk ρ e)
-  | Untyped.witness e p => Untyped.witness (wk ρ e) (wk ρ p)
-  | Untyped.let_wit p => Untyped.let_wit (wk (Wk.liftn 2 ρ) p)
-  | Untyped.refl e => Untyped.refl (wk ρ e)
+  | nil
+  | abort (p: RawUntyped)
+  | conj (l: RawUntyped) (r: RawUntyped)
+  | comp (b: Bool) (p: RawUntyped)
+  | disj (b: Bool) (p: RawUntyped)
+  | case_pr (p: RawUntyped) (l: RawUntyped) (r: RawUntyped)
+  | imp (φ: RawUntyped) (p: RawUntyped)
+  | mp (l: RawUntyped) (r: RawUntyped)
+  | general (A: RawUntyped) (p: RawUntyped)
+  | inst (p: RawUntyped) (e: RawUntyped)
+  | witness (e: RawUntyped) (p: RawUntyped)
+  | let_wit (p: RawUntyped)
+  | refl (e: RawUntyped)
 
---TODO: shorten...
-@[simp] theorem wk_comp (ρ: Wk n m) (σ: Wk m l): (u: Untyped l) -> wk ρ (wk σ u) = wk (Wk.comp ρ σ) u
+notation "genRecRawUntyped" u "=>" var "," r => match u with
+  | RawUntyped.var v => var v
+
+  | RawUntyped.nats => r UntypedKind.nats
+  | RawUntyped.pi A B => r UntypedKind.pi, 0, A, 1, B
+  | RawUntyped.sigma A B => r UntypedKind.sigma, 0, A, 1, B
+  | RawUntyped.coprod A B => r UntypedKind.coprod, 0, A, 0, B
+  | RawUntyped.set A φ => r UntypedKind.set, 0, A, 1, φ
+  | RawUntyped.assume φ A => r UntypedKind.assume, 0, φ, 0, A
+  | RawUntyped.intersect A B => r UntypedKind.intersect, 0, A, 1, B
+  | RawUntyped.union A B => r UntypedKind.union, 0, A, 1, B
+
+  | RawUntyped.top φ ψ => r UntypedKind.top
+  | RawUntyped.bot φ ψ => r UntypedKind.bot
+  | RawUntyped.and φ ψ => r UntypedKind.and, 0, φ, 0, ψ
+  | RawUntyped.or φ ψ => r UntypedKind.or, 0, φ, 0, ψ
+  | RawUntyped.implies φ Ψ => r UntypedKind.implies, 0, φ, 0, ψ
+  | RawUntyped.forall_ A φ => r UntypedKind.forall_, 0, A, 1, φ
+  | RawUntyped.exists_ A φ => r UntypedKind.exists_, 0, A, 1, φ
+  | RawUntyped.eq A e e' => r UntypedKind.exists, 0, A, 0, e, 0, e'
   
-  -- Variables
-  | Untyped.var _ => by simp [wk]
-  
-  -- Types
-  | Untyped.nat => rfl
-  | Untyped.pi A B => by { simp only [wk]; simp only [wk_comp, wk_lift_comp] }
-  | Untyped.sigma A B => by { simp only [wk]; simp only [wk_comp, wk_lift_comp] }
-  | Untyped.coprod A B => by { simp only [wk]; simp only [wk_comp, wk_lift_comp] }
-  | Untyped.set A B => by { simp only [wk]; simp only [wk_comp, wk_lift_comp] }
-  | Untyped.assume φ A => by { simp only [wk]; simp only [wk_comp, wk_lift_comp] }
-  | Untyped.intersect A B => by { simp only [wk]; simp only [wk_comp, wk_lift_comp] }
-  | Untyped.union A B => by { simp only [wk]; simp only [wk_comp, wk_lift_comp] }
+  | RawUntyped.nat n => r (UntypedKind.nat n)
+  | RawUntyped.lam A e => r UntypedKind.lam, 0, A, 1, e
+  | RawUntyped.app l r => r UntypedKind.app, 0, l, 0, r
+  | RawUntyped.pair l r => r UntypedKind.pair, 0, l, 0, r
+  | RawUntyped.proj b e => r (UntypedKind.proj b), 0, e
+  | RawUntyped.inj b e => r (UntypedKind.inj b), 0, e
+  | RawUntyped.case e l r => r (UntypedKind.case), 0, e, 0, l, 0, r
+  | RawUntyped.mkset e p => r (UntypedKind.mkset), 0, e, 1, p
+  | RawUntyped.letset e => r (UntypedKind.letset), 2, e
+  | RawUntyped.lam_pr φ e => r (UntypedKind.lam_pr), 0, φ, 1, e
+  | RawUntyped.app_pr e p => r (UntypedKind.app_pr), 0, e, 0, p
+  | RawUntyped.lam_irrel A e => r (UntypedKind.lam_irrel), 0, A, 1, e
+  | RawUntyped.app_irrel l r => r (UntypedKind.app_irrel), 0, l, 0, r
+  | RawUntyped.repr l r => r (UntypedKind.repr), 0, l, 0, r
+  | RawUntyped.let_repr e => r (UntypedKind.let_repr), 2, e
 
-  -- Propositions
-  | Untyped.top => rfl
-  | Untyped.bot => rfl
-  | Untyped.and φ ψ => by { simp only [wk]; simp only [wk_comp, wk_lift_comp] }  
-  | Untyped.or φ ψ => by { simp only [wk]; simp only [wk_comp, wk_lift_comp] }  
-  | Untyped.implies φ ψ => by { simp only [wk]; simp only [wk_comp, wk_lift_comp] }  
-  | Untyped.forall_ A φ => by { simp only [wk]; simp only [wk_comp, wk_lift_comp] }  
-  | Untyped.exists_ A φ => by { simp only [wk]; simp only [wk_comp, wk_lift_comp] }  
-  | Untyped.eq A l r => by { simp only [wk]; simp only [wk_comp, wk_lift_comp] }  
-  
-  -- Terms
-  | Untyped.lam A e => by { simp only [wk]; simp only [wk_comp, wk_lift_comp] }  
-  | Untyped.app l r => by { simp only [wk]; simp only [wk_comp, wk_lift_comp] }  
-  | Untyped.pair l r => by { simp only [wk]; simp only [wk_comp, wk_lift_comp] }  
-  | Untyped.proj b e => by { simp only [wk]; simp only [wk_comp, wk_lift_comp] }  
-  | Untyped.inj b e => by { simp only [wk]; simp only [wk_comp, wk_lift_comp] }  
-  | Untyped.case e l r => by { simp only [wk]; simp only [wk_comp, wk_lift_comp] }  
-  | Untyped.mkset e p => by { simp only [wk]; simp only [wk_comp, wk_lift_comp] }  
-  | Untyped.letset e => by { simp only [wk, Wk.liftn]; simp only [wk_comp, wk_lift_comp] }  
-  | Untyped.lam_pr φ e => by { simp only [wk]; simp only [wk_comp, wk_lift_comp] }  
-  | Untyped.app_pr φ e => by { simp only [wk]; simp only [wk_comp, wk_lift_comp] }  
-  | Untyped.lam_irrel l r => by { simp only [wk]; simp only [wk_comp, wk_lift_comp] }  
-  | Untyped.app_irrel l r => by { simp only [wk]; simp only [wk_comp, wk_lift_comp] }  
-  | Untyped.repr l r => by { simp only [wk]; simp only [wk_comp, wk_lift_comp] }  
-  | Untyped.let_repr e => by { simp only [wk, Wk.liftn]; simp only [wk_comp, wk_lift_comp] }  
+  | RawUntyped.nil => r (UntypedKind.nil)
+  | RawUntyped.abort p => r (UntypedKind.abort), 0, p
+  | RawUntyped.conj l r => r (UntypedKind.conj), 0, l, 0, r
+  | RawUntyped.comp b p => r (UntypedKind.comp b), 0, p
+  | RawUntyped.disj b p => r (UntypedKind.disj b), 0, p
+  | RawUntyped.case_pr p l r => r (UntypedKind.case_pr), 0, p, 0, l, 0, r
+  | RawUntyped.imp φ p => r (UntypedKind.imp), φ, p
+  | RawUntyped.mp l r => r (UntypedKind.mp), 0, l, 0, r
+  | RawUntyped.general A p => r (UntypedKind.general), 0, A, 1, p
+  | RawUntyped.inst p e => r (UntypedKind.inst), 0, p, 0, e
+  | RawUntyped.witness e p => r (UntypedKind.witness), 0, e, 0, p
+  | RawUntyped.let_wit p => r (UntypedKind.let_wit), 2, p
+  | RawUntyped.refl e => r (UntypedKind.refl), 0, e
 
-  -- Proofs
-  | Untyped.nil => rfl
-  | Untyped.abort p => by { simp only [wk]; simp only [wk_comp, wk_lift_comp] }  
-  | Untyped.conj l r => by { simp only [wk]; simp only [wk_comp, wk_lift_comp] }  
-  | Untyped.comp b p => by { simp only [wk]; simp only [wk_comp, wk_lift_comp] }  
-  | Untyped.disj b p => by { simp only [wk]; simp only [wk_comp, wk_lift_comp] }  
-  | Untyped.case_pr p l r => by { simp only [wk]; simp only [wk_comp, wk_lift_comp] }  
-  | Untyped.imp φ p => by { simp only [wk]; simp only [wk_comp, wk_lift_comp] }  
-  | Untyped.mp l r => by { simp only [wk]; simp only [wk_comp, wk_lift_comp] }  
-  | Untyped.general A p => by { simp only [wk]; simp only [wk_comp, wk_lift_comp] }  
-  | Untyped.inst p e => by { simp only [wk]; simp only [wk_comp, wk_lift_comp] }  
-  | Untyped.witness e p => by { simp only [wk]; simp only [wk_comp, wk_lift_comp] }  
-  | Untyped.let_wit p => by { simp only [wk, Wk.liftn]; simp only [wk_comp, wk_lift_comp] }  
-  | Untyped.refl e => by { simp only [wk]; simp only [wk_comp, wk_lift_comp] }  
-
-def Subst (m: Nat) (n: Nat): Type 0 := Fin n -> Untyped m
-
-@[simp] def Subst.head (σ: Subst m (Nat.succ n)): Untyped m := σ Fin.zero
-
-def Subst.tail (σ: Subst m (Nat.succ n)): Subst m n :=  λv => σ (Fin.succ v)
-
-def Subst.id: Subst n n := Untyped.var
-
-def Subst.wk1 (σ: Subst m n): Subst (m + 1) n := λ x => wk Wk.wk1 (σ x)
-
-def Subst.lift (σ: Subst m n): Subst (m + 1) (n + 1)
-  | Fin.mk 0 p => Untyped.var Fin.zero
-  | Fin.mk (Nat.succ n) p => Subst.wk1 σ (Fin.mk n (Nat.lt_of_succ_lt_succ p))
-
-@[simp] def Subst.liftn: (l: Nat) -> Subst m n -> Subst (m + l) (n + l)
-  | 0, σ => σ
-  | Nat.succ n, σ => Subst.lift (liftn n σ)
-
-def toSubst (ρ: Wk m n): Subst m n := λv => Untyped.var (Wk.var ρ v)
-
-instance {m n: Nat}: Coe (Wk m n) (Subst m n) where
-  coe w := toSubst w
-
-@[simp] def Subst.cons (σ: Subst m n) (t: Untyped m): Subst m (n + 1)
-  | (Fin.mk 0 _) => t
-  | (Fin.mk (Nat.succ n) p) => σ (Fin.mk n (Nat.lt_of_succ_lt_succ p))
-
-@[simp] def Subst.sg: Untyped n -> Subst n (n + 1) := Subst.cons Subst.id
-
-@[simp] def subst (σ: Subst m n): Untyped n -> Untyped m
-
-  -- Variables
-  | Untyped.var v => σ v
-
-  -- Types
-  | Untyped.nat => Untyped.nat
-  | Untyped.pi A B => Untyped.pi (subst σ A) (subst (Subst.lift σ) B)
-  | Untyped.sigma A B => Untyped.sigma (subst σ A) (subst (Subst.lift σ) B)
-  | Untyped.coprod A B => Untyped.coprod (subst σ A) (subst σ B)
-  | Untyped.set A φ => Untyped.set (subst σ A) (subst (Subst.lift σ) φ)
-  | Untyped.assume φ A => Untyped.assume (subst σ φ) (subst σ A)
-  | Untyped.intersect A B => Untyped.intersect (subst σ A) (subst (Subst.lift σ) B)
-  | Untyped.union A B => Untyped.union (subst σ A) (subst (Subst.lift σ) B)
-
-  -- Propositions
-  | Untyped.top => Untyped.top
-  | Untyped.bot => Untyped.bot
-  | Untyped.and φ ψ => Untyped.and (subst σ φ) (subst σ ψ)
-  | Untyped.or φ ψ => Untyped.or (subst σ φ) (subst σ ψ)
-  | Untyped.implies φ ψ => Untyped.implies (subst σ φ) (subst σ ψ)
-  | Untyped.forall_ A φ => Untyped.forall_ (subst σ A) (subst (Subst.lift σ) φ)
-  | Untyped.exists_ A φ => Untyped.exists_ (subst σ A) (subst (Subst.lift σ) φ)
-  | Untyped.eq A l r => Untyped.eq (subst σ A) (subst σ l) (subst σ r)
-  
-  -- Terms
-  | Untyped.lam A e => Untyped.lam (subst σ A) (subst (Subst.lift σ) e)
-  | Untyped.app l r => Untyped.app (subst σ l) (subst σ r)
-  | Untyped.pair l r => Untyped.pair (subst σ l) (subst σ r)
-  | Untyped.proj b e => Untyped.proj b (subst σ e)
-  | Untyped.inj b e => Untyped.inj b (subst σ e)
-  | Untyped.case e l r => Untyped.case (subst σ e) (subst σ l) (subst σ r)
-  | Untyped.mkset e p => Untyped.mkset (subst σ e) (subst σ p)
-  | Untyped.letset e => Untyped.letset (subst (Subst.liftn 2 σ) e)
-  | Untyped.lam_pr φ e => Untyped.lam_pr (subst σ φ) (subst (Subst.lift σ) e)
-  | Untyped.app_pr φ e => Untyped.app_pr (subst σ φ) (subst σ e)
-  | Untyped.lam_irrel l r => Untyped.lam_irrel (subst σ l) (subst (Subst.lift σ) r)
-  | Untyped.app_irrel l r => Untyped.app_irrel (subst σ l) (subst σ r)
-  | Untyped.repr l r => Untyped.repr (subst σ l) (subst σ r)
-  | Untyped.let_repr e => Untyped.let_repr (subst (Subst.liftn 2 σ) e)
-
-  -- Proofs
-  | Untyped.nil => Untyped.nil
-  | Untyped.abort p => Untyped.abort (subst σ p)
-  | Untyped.conj l r => Untyped.conj (subst σ l) (subst σ r)
-  | Untyped.comp b p => Untyped.comp b (subst σ p)
-  | Untyped.disj b p => Untyped.disj b (subst σ p)
-  | Untyped.case_pr p l r => Untyped.case_pr (subst σ p) (subst σ l) (subst σ r)
-  | Untyped.imp φ p => Untyped.imp (subst σ φ) (subst (Subst.lift σ) p)
-  | Untyped.mp l r => Untyped.mp (subst σ l) (subst σ r)
-  | Untyped.general A p => Untyped.general (subst σ A) (subst (Subst.lift σ) p)
-  | Untyped.inst p e => Untyped.inst (subst σ p) (subst σ e)
-  | Untyped.witness e p => Untyped.witness (subst σ e) (subst σ p)
-  | Untyped.let_wit p => Untyped.let_wit (subst (Subst.liftn 2 σ) p)
-  | Untyped.refl e => Untyped.refl (subst σ e)
-
-def Subst.comp (σ: Subst l m) (τ: Subst m n): Subst l n :=
-  λv => subst σ (τ v)
-
-private theorem subst_wk_lift_inner (ρ: Wk n m): (v: Fin (m + 1)) -> 
-  Subst.lift (toSubst ρ) v = toSubst (Wk.lift ρ) v
-  | Fin.mk 0 _ => by simp [Subst.lift, toSubst]
-  | Fin.mk (Nat.succ n) _ => by simp [Subst.lift, Subst.wk1, toSubst, wk]
-  
-@[simp] theorem subst_wk_lift (ρ: Wk n m):
-  Subst.lift (toSubst ρ) = toSubst (Wk.lift ρ) := by {
-    funext v;
-    apply subst_wk_lift_inner
-  }
-
-private theorem subst_wk_inner (ρ: Wk n m): (u: Untyped m) -> subst ρ u = wk ρ u
-
-  -- Variables
-  | Untyped.var _ => by simp [subst, wk, toSubst]
-  
-  -- Types
-  | Untyped.nat => rfl
-  | Untyped.pi A B => by { simp only [subst]; simp only [subst_wk_lift, wk, subst_wk_inner] }  
-  | Untyped.sigma A B => by { simp only [subst]; simp only [subst_wk_lift, wk, subst_wk_inner] }  
-  | Untyped.coprod A B => by { simp only [subst]; simp only [subst_wk_lift, wk, subst_wk_inner] }  
-  | Untyped.set A B => by { simp only [subst]; simp only [subst_wk_lift, wk, subst_wk_inner] }  
-  | Untyped.assume φ A => by { simp only [subst]; simp only [subst_wk_lift, wk, subst_wk_inner] }  
-  | Untyped.intersect A B => by { simp only [subst]; simp only [subst_wk_lift, wk, subst_wk_inner] }  
-  | Untyped.union A B => by { simp only [subst]; simp only [subst_wk_lift, wk, subst_wk_inner] }  
-
-  -- Propositions
-  | Untyped.top => rfl
-  | Untyped.bot => rfl
-  | Untyped.and φ ψ => by { simp only [subst]; simp only [subst_wk_lift, wk, subst_wk_inner] }    
-  | Untyped.or φ ψ => by { simp only [subst]; simp only [subst_wk_lift, wk, subst_wk_inner] }    
-  | Untyped.implies φ ψ => by { simp only [subst]; simp only [subst_wk_lift, wk, subst_wk_inner] }    
-  | Untyped.forall_ A φ => by { simp only [subst]; simp only [subst_wk_lift, wk, subst_wk_inner] }    
-  | Untyped.exists_ A φ => by { simp only [subst]; simp only [subst_wk_lift, wk, subst_wk_inner] }    
-  | Untyped.eq A l r => by { simp only [subst]; simp only [subst_wk_lift, wk, subst_wk_inner] }    
-  
-  -- Terms
-  | Untyped.lam A e => by { simp only [subst]; simp only [subst_wk_lift, wk, subst_wk_inner] }    
-  | Untyped.app l r => by { simp only [subst]; simp only [subst_wk_lift, wk, subst_wk_inner] }    
-  | Untyped.pair l r => by { simp only [subst]; simp only [subst_wk_lift, wk, subst_wk_inner] }    
-  | Untyped.proj b e => by { simp only [subst]; simp only [subst_wk_lift, wk, subst_wk_inner] }    
-  | Untyped.inj b e => by { simp only [subst]; simp only [subst_wk_lift, wk, subst_wk_inner] }    
-  | Untyped.case e l r => by { simp only [subst]; simp only [subst_wk_lift, wk, subst_wk_inner] }    
-  | Untyped.mkset e p => by { simp only [subst]; simp only [subst_wk_lift, wk, subst_wk_inner] }  
-  | Untyped.letset e => 
-    by { simp only [subst, Subst.liftn]; simp only [Wk.liftn, subst_wk_lift, wk, subst_wk_inner] }  
-  | Untyped.lam_pr φ e => by { simp only [subst]; simp only [subst_wk_lift, wk, subst_wk_inner] }    
-  | Untyped.app_pr φ e => by { simp only [subst]; simp only [subst_wk_lift, wk, subst_wk_inner] }    
-  | Untyped.lam_irrel l r => by { simp only [subst]; simp only [subst_wk_lift, wk, subst_wk_inner] }    
-  | Untyped.app_irrel l r => by { simp only [subst]; simp only [subst_wk_lift, wk, subst_wk_inner] }    
-  | Untyped.repr l r => by { simp only [subst]; simp only [subst_wk_lift, wk, subst_wk_inner] }    
-  | Untyped.let_repr e => 
-    by { simp only [subst, Subst.liftn]; simp only [Wk.liftn, subst_wk_lift, wk, subst_wk_inner] }  
-
-  -- Proofs
-  | Untyped.nil => rfl
-  | Untyped.abort p => by { simp only [subst]; simp only [subst_wk_lift, wk, subst_wk_inner] }    
-  | Untyped.conj l r => by { simp only [subst]; simp only [subst_wk_lift, wk, subst_wk_inner] }    
-  | Untyped.comp b p => by { simp only [subst]; simp only [subst_wk_lift, wk, subst_wk_inner] }    
-  | Untyped.disj b p => by { simp only [subst]; simp only [subst_wk_lift, wk, subst_wk_inner] }    
-  | Untyped.case_pr p l r => by { simp only [subst]; simp only [subst_wk_lift, wk, subst_wk_inner] }    
-  | Untyped.imp φ p => by { simp only [subst]; simp only [subst_wk_lift, wk, subst_wk_inner] }    
-  | Untyped.mp l r => by { simp only [subst]; simp only [subst_wk_lift, wk, subst_wk_inner] }    
-  | Untyped.general A p => by { simp only [subst]; simp only [subst_wk_lift, wk, subst_wk_inner] }    
-  | Untyped.inst p e => by { simp only [subst]; simp only [subst_wk_lift, wk, subst_wk_inner] }    
-  | Untyped.witness e p => by { simp only [subst]; simp only [subst_wk_lift, wk, subst_wk_inner] }    
-  | Untyped.let_wit p => 
-    by { simp only [subst, Subst.liftn]; simp only [Wk.liftn, subst_wk_lift, wk, subst_wk_inner] }  
-  | Untyped.refl e => by { simp only [subst]; simp only [subst_wk_lift, wk, subst_wk_inner] }    
-
-theorem subst_wk (ρ: Wk n m): subst ρ = wk ρ := by {
-  funext u;
-  apply subst_wk_inner
-}
-
-def Wk.wk_liftn (l: Nat): Wk (m + (l + 1)) (m + l) := by {
-  have a: (m + (l + 1)) = m + 1 + l := sorry;
-  rw [a];
-  exact (Wk.liftn l Wk.wk1)
-}
-
-@[simp] theorem subst_wk1_liftn (σ: Subst n m): (l: Nat) -> (u: Untyped (m + l)) -> 
-  subst (Subst.liftn (l + 1) σ) (wk (Wk.wk_liftn l) u) = wk (Wk.wk_liftn l) (subst (Subst.liftn l σ) u)
-
-  -- Variables
-  | _, Untyped.var (Fin.mk 0 _) => sorry
-  | _, Untyped.var (Fin.mk (Nat.succ n) _) => sorry
-
-  -- Types
-  | _, Untyped.nat => sorry
-  | _, Untyped.pi A B => sorry
-  
-  | _, _ => sorry
-  -- | Untyped.sigma A B => by { simp only [subst]; simp only [subst_wk_lift, wk, subst_wk_inner] }  
-  -- | Untyped.coprod A B => by { simp only [subst]; simp only [subst_wk_lift, wk, subst_wk_inner] }  
-  -- | Untyped.set A B => by { simp only [subst]; simp only [subst_wk_lift, wk, subst_wk_inner] }  
-  -- | Untyped.assume φ A => by { simp only [subst]; simp only [subst_wk_lift, wk, subst_wk_inner] }  
-  -- | Untyped.intersect A B => by { simp only [subst]; simp only [subst_wk_lift, wk, subst_wk_inner] }  
-  -- | Untyped.union A B => by { simp only [subst]; simp only [subst_wk_lift, wk, subst_wk_inner] }  
-
-  -- -- Propositions
-  -- | Untyped.top => rfl
-  -- | Untyped.bot => rfl
-  -- | Untyped.and φ ψ => by { simp only [subst]; simp only [subst_wk_lift, wk, subst_wk_inner] }    
-  -- | Untyped.or φ ψ => by { simp only [subst]; simp only [subst_wk_lift, wk, subst_wk_inner] }    
-  -- | Untyped.implies φ ψ => by { simp only [subst]; simp only [subst_wk_lift, wk, subst_wk_inner] }    
-  -- | Untyped.forall_ A φ => by { simp only [subst]; simp only [subst_wk_lift, wk, subst_wk_inner] }    
-  -- | Untyped.exists_ A φ => by { simp only [subst]; simp only [subst_wk_lift, wk, subst_wk_inner] }    
-  -- | Untyped.eq A l r => by { simp only [subst]; simp only [subst_wk_lift, wk, subst_wk_inner] }    
-  
-  -- -- Terms
-  -- | Untyped.lam A e => by { simp only [subst]; simp only [subst_wk_lift, wk, subst_wk_inner] }    
-  -- | Untyped.app l r => by { simp only [subst]; simp only [subst_wk_lift, wk, subst_wk_inner] }    
-  -- | Untyped.pair l r => by { simp only [subst]; simp only [subst_wk_lift, wk, subst_wk_inner] }    
-  -- | Untyped.proj b e => by { simp only [subst]; simp only [subst_wk_lift, wk, subst_wk_inner] }    
-  -- | Untyped.inj b e => by { simp only [subst]; simp only [subst_wk_lift, wk, subst_wk_inner] }    
-  -- | Untyped.case e l r => by { simp only [subst]; simp only [subst_wk_lift, wk, subst_wk_inner] }    
-  -- | Untyped.mkset e p => by { simp only [subst]; simp only [subst_wk_lift, wk, subst_wk_inner] }  
-  -- | Untyped.letset e => 
-  --   by { simp only [subst, Subst.liftn]; simp only [Wk.liftn, subst_wk_lift, wk, subst_wk_inner] }  
-  -- | Untyped.lam_pr φ e => by { simp only [subst]; simp only [subst_wk_lift, wk, subst_wk_inner] }    
-  -- | Untyped.app_pr φ e => by { simp only [subst]; simp only [subst_wk_lift, wk, subst_wk_inner] }    
-  -- | Untyped.lam_irrel l r => by { simp only [subst]; simp only [subst_wk_lift, wk, subst_wk_inner] }    
-  -- | Untyped.app_irrel l r => by { simp only [subst]; simp only [subst_wk_lift, wk, subst_wk_inner] }    
-  -- | Untyped.repr l r => by { simp only [subst]; simp only [subst_wk_lift, wk, subst_wk_inner] }    
-  -- | Untyped.let_repr e => 
-  --   by { simp only [subst, Subst.liftn]; simp only [Wk.liftn, subst_wk_lift, wk, subst_wk_inner] }  
-
-  -- -- Proofs
-  -- | Untyped.nil => rfl
-  -- | Untyped.abort p => by { simp only [subst]; simp only [subst_wk_lift, wk, subst_wk_inner] }    
-  -- | Untyped.conj l r => by { simp only [subst]; simp only [subst_wk_lift, wk, subst_wk_inner] }    
-  -- | Untyped.comp b p => by { simp only [subst]; simp only [subst_wk_lift, wk, subst_wk_inner] }    
-  -- | Untyped.disj b p => by { simp only [subst]; simp only [subst_wk_lift, wk, subst_wk_inner] }    
-  -- | Untyped.case_pr p l r => by { simp only [subst]; simp only [subst_wk_lift, wk, subst_wk_inner] }    
-  -- | Untyped.imp φ p => by { simp only [subst]; simp only [subst_wk_lift, wk, subst_wk_inner] }    
-  -- | Untyped.mp l r => by { simp only [subst]; simp only [subst_wk_lift, wk, subst_wk_inner] }    
-  -- | Untyped.general A p => by { simp only [subst]; simp only [subst_wk_lift, wk, subst_wk_inner] }    
-  -- | Untyped.inst p e => by { simp only [subst]; simp only [subst_wk_lift, wk, subst_wk_inner] }    
-  -- | Untyped.witness e p => by { simp only [subst]; simp only [subst_wk_lift, wk, subst_wk_inner] }    
-  -- | Untyped.let_wit p => 
-  --   by { simp only [subst, Subst.liftn]; simp only [Wk.liftn, subst_wk_lift, wk, subst_wk_inner] }  
-  -- | Untyped.refl e => by { simp only [subst]; simp only [subst_wk_lift, wk, subst_wk_inner] }    
-
-
-@[simp] theorem subst_wk1_lift (σ: Subst n m) (u: Untyped m):
-  subst (Subst.lift σ) (wk Wk.wk1 u) = wk Wk.wk1 (subst σ u) := subst_wk1_liftn σ 0 u
-
-@[simp] theorem subst_lift_comp (σ: Subst n m) (τ: Subst m l):
-  Subst.comp (Subst.lift σ) (Subst.lift τ) = Subst.lift (Subst.comp σ τ) := by {
-    funext (Fin.mk v p);
-    simp [Subst.comp];
-    cases v with
-    | zero => rfl
-    | succ v => 
-      simp [Subst.lift, Subst.wk1];
-      rw [←subst_wk1_lift];
-      rfl
-  }
-
---TODO: shorten...
-@[simp] theorem subst_comp (σ: Subst n m) (τ: Subst m l): (u: Untyped l) -> 
-  subst σ (subst τ u) = subst (Subst.comp σ τ) u
-  -- Variables
-  | Untyped.var _ => by simp [Subst.comp, subst]
-  
-  -- Types
-  | Untyped.nat => rfl
-  | Untyped.pi A B => by { simp only [subst]; simp only [subst_comp, subst_lift_comp] }
-  | Untyped.sigma A B => by { simp only [subst]; simp only [subst_comp, subst_lift_comp] }
-  | Untyped.coprod A B => by { simp only [subst]; simp only [subst_comp, subst_lift_comp] }
-  | Untyped.set A B => by { simp only [subst]; simp only [subst_comp, subst_lift_comp] }
-  | Untyped.assume φ A => by { simp only [subst]; simp only [subst_comp, subst_lift_comp] }
-  | Untyped.intersect A B => by { simp only [subst]; simp only [subst_comp, subst_lift_comp] }
-  | Untyped.union A B => by { simp only [subst]; simp only [subst_comp, subst_lift_comp] }
-
-  -- Propositions
-  | Untyped.top => rfl
-  | Untyped.bot => rfl
-  | Untyped.and φ ψ => by { simp only [subst]; simp only [subst_comp, subst_lift_comp] }  
-  | Untyped.or φ ψ => by { simp only [subst]; simp only [subst_comp, subst_lift_comp] }  
-  | Untyped.implies φ ψ => by { simp only [subst]; simp only [subst_comp, subst_lift_comp] }  
-  | Untyped.forall_ A φ => by { simp only [subst]; simp only [subst_comp, subst_lift_comp] }  
-  | Untyped.exists_ A φ => by { simp only [subst]; simp only [subst_comp, subst_lift_comp] }  
-  | Untyped.eq A l r => by { simp only [subst]; simp only [subst_comp, subst_lift_comp] }  
-  
-  -- Terms
-  | Untyped.lam A e => by { simp only [subst]; simp only [subst_comp, subst_lift_comp] }  
-  | Untyped.app l r => by { simp only [subst]; simp only [subst_comp, subst_lift_comp] }  
-  | Untyped.pair l r => by { simp only [subst]; simp only [subst_comp, subst_lift_comp] }  
-  | Untyped.proj b e => by { simp only [subst]; simp only [subst_comp, subst_lift_comp] }  
-  | Untyped.inj b e => by { simp only [subst]; simp only [subst_comp, subst_lift_comp] }  
-  | Untyped.case e l r => by { simp only [subst]; simp only [subst_comp, subst_lift_comp] }  
-  | Untyped.mkset e p => by { simp only [subst]; simp only [subst_comp, subst_lift_comp] }  
-  | Untyped.letset e => by { simp only [subst, Subst.liftn]; simp only [subst_comp, subst_lift_comp] }  
-  | Untyped.lam_pr φ e => by { simp only [subst]; simp only [subst_comp, subst_lift_comp] }  
-  | Untyped.app_pr φ e => by { simp only [subst]; simp only [subst_comp, subst_lift_comp] }  
-  | Untyped.lam_irrel l r => by { simp only [subst]; simp only [subst_comp, subst_lift_comp] }  
-  | Untyped.app_irrel l r => by { simp only [subst]; simp only [subst_comp, subst_lift_comp] }  
-  | Untyped.repr l r => by { simp only [subst]; simp only [subst_comp, subst_lift_comp] }  
-  | Untyped.let_repr e => by { simp only [subst, Subst.liftn]; simp only [subst_comp, subst_lift_comp] }  
-
-  -- Proofs
-  | Untyped.nil => rfl
-  | Untyped.abort p => by { simp only [subst]; simp only [subst_comp, subst_lift_comp] }  
-  | Untyped.conj l r => by { simp only [subst]; simp only [subst_comp, subst_lift_comp] }  
-  | Untyped.comp b p => by { simp only [subst]; simp only [subst_comp, subst_lift_comp] }  
-  | Untyped.disj b p => by { simp only [subst]; simp only [subst_comp, subst_lift_comp] }  
-  | Untyped.case_pr p l r => by { simp only [subst]; simp only [subst_comp, subst_lift_comp] }  
-  | Untyped.imp φ p => by { simp only [subst]; simp only [subst_comp, subst_lift_comp] }  
-  | Untyped.mp l r => by { simp only [subst]; simp only [subst_comp, subst_lift_comp] }  
-  | Untyped.general A p => by { simp only [subst]; simp only [subst_comp, subst_lift_comp] }  
-  | Untyped.inst p e => by { simp only [subst]; simp only [subst_comp, subst_lift_comp] }  
-  | Untyped.witness e p => by { simp only [subst]; simp only [subst_comp, subst_lift_comp] }  
-  | Untyped.let_wit p => by { simp only [subst, Subst.liftn]; simp only [subst_comp, subst_lift_comp] }  
-  | Untyped.refl e => by { simp only [subst]; simp only [subst_comp, subst_lift_comp] }  
